SStructTT/Static/Context.lean
@@ -7,4 +7,4 @@ inductive Has {Srt} : Ctx Srt -> Var -> Tm Srt -> Prop where
     Has (A :: Γ) 0 A.[shift 1]
   | succ Γ A B x :
     Has Γ x A ->
-    Has (B :: Γ) x.succ A.[shift 1]
+    Has (B :: Γ) (x + 1) A.[shift 1]
