SStructTT/Static/Renaming.lean
@@ -1,0 +1,16 @@
+import SStructTT.Static.Typed
+
+namespace Static
+variable {Srt : Type} [SStruct Srt]
+
+inductive AgreeRen : (Var -> Var) -> Ctx Srt -> Ctx Srt -> Prop where
+  | nil {ξ} :
+    AgreeRen ξ  [] []
+  | cons Γ Γ' A s i ξ :
+    Typed Γ A (.srt s i) ->
+    AgreeRen ξ Γ Γ' ->
+    AgreeRen (upren ξ) (A :: Γ) (A.[ren ξ] :: Γ')
+  | wk Γ Γ' A s i ξ :
+    Typed Γ' A (.srt s i) ->
+    AgreeRen ξ Γ Γ' ->
+    AgreeRen (ξ !>> (.+1)) Γ (A :: Γ')
