SStructTT/Static/Typed.lean
@@ -8,68 +8,68 @@ variable {Srt : Type} [SStruct Srt]
 
 mutual
 inductive Typed : Ctx Srt -> Tm Srt -> Tm Srt -> Prop where
-  | srt Γ i :
+  | srt {Γ} i :
     Wf Γ ->
-    Typed Γ (.srt s0 i) (.srt s0 (i.succ))
-  | var Γ x A :
+    Typed Γ (.srt s0 i) (.srt s0 (i + 1))
+  | var {Γ x A} :
     Wf Γ ->
     Has Γ x A ->
     Typed Γ (.var x) A
-  | pi Γ A B r s sA sB iA iB :
+  | pi {Γ A B} r s {sA sB iA iB} :
     Typed Γ A (.srt sA iA) ->
     Typed (A :: Γ) B (.srt sB iB) ->
     Typed Γ (.pi A B r s) (.srt s (max iA iB))
-  | lam Γ A B m r s sA iA :
+  | lam {Γ A B m} r s {sA iA} :
     Typed Γ A (.srt sA iA) ->
     Typed (A :: Γ) m B ->
     Typed Γ (.lam A m r s) (.pi A B r s)
-  | app Γ A B m n r s :
+  | app {Γ A B m n r s} :
     Typed Γ m (.pi A B r s) ->
     Typed Γ n A ->
     Typed Γ (.app m n) B.[n/]
-  | sig Γ A B r s sA sB iA iB :
+  | sig {Γ A B} r s {sA sB iA iB} :
     Typed Γ A (.srt sA iA) ->
     Typed (A :: Γ) B (.srt sB iB) ->
     Typed Γ (.sig A B r s) (.srt s (max iA iB))
-  | pair Γ A B m n r s i :
+  | pair {Γ A B m n r s i} :
     Typed Γ (.pi A B r s) (.srt s i) ->
     Typed Γ m A ->
     Typed Γ n B.[m/] ->
     Typed Γ (.pair m n r s) (.sig A B r s)
-  | proj Γ A B C m n r s sC iC :
+  | proj {Γ A B C m n r s sC iC} :
     Typed (.sig A B r s :: Γ) C (.srt sC iC) ->
     Typed Γ m (.sig A B r s) ->
     Typed (B :: A :: Γ) n C.[.pair (.var 1) (.var 0) r s .: shift 2] ->
     Typed Γ (.proj C m n) C.[m/]
-  | bool Γ :
+  | bool {Γ} :
     Wf Γ ->
     Typed Γ .bool (.srt s0 0)
-  | tt Γ :
+  | tt {Γ} :
     Wf Γ ->
     Typed Γ .tt .bool
-  | ff Γ :
+  | ff {Γ} :
     Wf Γ ->
     Typed Γ .ff .bool
-  | ite Γ A m n1 n2 s i :
+  | ite {Γ A m n1 n2 s i} :
     Typed (.bool :: Γ) A (.srt s i) ->
     Typed Γ m .bool ->
     Typed Γ n1 A.[.tt/] ->
     Typed Γ n2 A.[.ff/] ->
     Typed Γ (.ite A m n1 n2) A.[m/]
-  | id Γ A m n s i :
+  | id {Γ A m n s i} :
     Typed Γ A (.srt s i) ->
     Typed Γ m A ->
     Typed Γ n A ->
     Typed Γ  (.id A m n) (.srt s0 i)
-  | rfl Γ A m :
+  | rfl {Γ A m} :
     Typed Γ m A ->
     Typed Γ (.rfl m) (.id A m m)
-  | rw Γ A B m n a b s i :
+  | rw {Γ A B m n a b s i} :
     Typed (.id A.[shift 1] a.[shift 1] (.var 0) :: A :: Γ) B (.srt s i) ->
     Typed Γ m B.[.rfl a,a/] ->
     Typed Γ n (.id A a b) ->
     Typed Γ (.rw B m n) B.[n,b/]
-  | conv Γ A B m s i :
+  | conv {Γ A B m s i} :
     A === B ->
     Typed Γ m A ->
     Typed Γ B (.srt s i) ->
@@ -77,7 +77,7 @@ inductive Typed : Ctx Srt -> Tm Srt -> Tm Srt -> Prop where
 
 inductive Wf : Ctx Srt -> Prop where
   | nil : Wf []
-  | cons Γ A s i :
+  | cons {Γ A s i} :
     Typed Γ A (.srt s i) ->
     Wf Γ ->
     Wf (A :: Γ)
